Final -- sorry bros

q2b.dfy
@@ -6,14 +6,115 @@ predicate divides(a: nat, b:nat)
     exists k: nat :: b == k * a
 }
 
-// Bezout identity lemma
-lemma bezout(p: nat, q: nat, x: int, y: int)
-    requires p != 0 && q != 0 
-    ensures p*x + q*y == gcd(p,q)
+predicate quotientRemainderPredicate(a: nat, b: nat, q: nat, r: nat)
+    requires b > 0
 {
-    // Proof of lemma
-    
+    a == (q * b) + r && 0 <= r < b
 }
+
+lemma quotientRemainder(a: nat, b: nat)
+    requires b > 1 && a >= 0
+    ensures exists q, r :: quotientRemainderPredicate(a, b, q, r)
+{
+    if a == 0 {
+        var q := 0;
+        var r := 0;
+        assert a == b*q + r;
+        assert quotientRemainderPredicate(a,b,q,r);
+
+    } else {
+        quotientRemainder(a-1, b);
+        var q: nat, r: nat :| r >= 0 && a-1 == b*q + r;
+
+        if r == b - 1 {
+            assert quotientRemainderPredicate(a, b, (q+1), 0);
+        } else if r < b - 1 {
+          assert quotientRemainderPredicate(a, b, q, r+1);
+        } 
+    }
+    
+    //Uniqueness
+    
+    var q0: nat, r0: nat :| 0 <= r0 < b && b*q0 + r0 == a;
+    var q1: nat, r1: nat :| 0 <= r1 < b && b*q1 + r1 == a;
+        
+    calc == {
+      b*(q0-q1);
+      r1-r0;
+    }
+    assert 0 <= b*(q0-q1) < b;
+    assert 0 <= q0-q1 < 1;
+    assert q0-q1==0;
+    assert q0 == q1;
+    calc == {
+      r1-r0;
+      b*(q0-q1);
+      b*0;
+      0;
+    }
+    assert r1-r0 == 0;
+    assert r1 == r0;
+}
+
+
+// Bezout identity lemma
+lemma bezout(a: nat, b: nat, x: int, y: int)
+    requires a > 0 && b > 0 
+    ensures a*x + b*y == gcd(a,b)
+{
+    var k :| 0 < k;
+    if b == 0 // BASE CASE
+    {
+        assert forall x :: x >= 1 ==> gcd(x, 0) == x;
+        assert a >= 1;
+        calc == {
+            gcd(a, 0);
+            gcd(a, b);
+        }
+        assert gcd(a, b) == a;
+        calc == {
+            gcd(a, b);
+            a;
+            (a*1) + (b*0);
+        }
+        var x, y :| a*x + b*y == a;
+        assert a*x + b*y == gcd(a, b);
+    }
+    else // INDUCTION STEP
+    {
+        // ASSUME FOR b, NOW PROVE FOR b + 1
+        bezout(a, b-1, x, y);
+        //var b' := b + 1;
+        quotientRemainder(a, b);
+        var q, r :| a == (q * b) + r;
+        assert r == a - (q * b);
+        var p := q*x + y;
+        calc == {
+            gcd(a, b);
+            a*x + (b)*y;
+            (q*b + r)*x + (b)*y;
+            q*b*x + r*x + b*y;
+            q*b*x + b*y + r*x;
+            b*((q*x) + y) + r*x;
+            r*x + b*((q*x) + y);
+            gcd(b, r);
+        }
+        var m, n :| b*m + r*n == gcd(b, r);
+        var x0 := n;
+        var y0 := (m - q*n);
+        calc == {
+            gcd(b, r);
+            b*m + r*n;
+            b*m + (a - (q * b))*n;
+            b*m + a*n - q*b*n;
+            a*n + b*(m - q*n);
+            a*x0 + b*y0;
+            gcd(a, b);
+        }
+        assert b > b-1;
+    }
+}
+
 
 lemma gcdDivides(a: nat, b: nat, k: nat)
     requires a > 0 && b > 0 && k > 0
